program_verification_tactics.thy
@@ -8,6 +8,7 @@ theory program_verification_tactics
     execution_invariants_s
     execution_invariants_unused
     program_proof_rules
+    crdt_specs
 begin
 
 context begin
@@ -115,6 +116,13 @@ lemma state_def_h1[simp]: "S' ::= S \<Longrightarrow>  ls_pc (the (localState S'
 lemma state_def_h2[simp]: "S' ::= S \<Longrightarrow>  (currentTransaction S' i = None) \<longleftrightarrow> (currentTransaction S i = None)"  by (auto simp add: Def_def)
 lemma state_def_currentProc[simp]: "S' ::= S \<Longrightarrow>  currentProc S' i = currentProc S i" by (auto simp add: Def_def)
 lemma state_def_currentTransaction[simp]: "S' ::= S \<Longrightarrow> currentTransaction S' i = currentTransaction S i"  by (auto simp add: Def_def)
+
+
+method show_procedures_cannot_guess_ids = 
+  (((auto simp add: newId_def bind_def atomic_def beginAtomic_def call_def skip_def endAtomic_def return_def 
+        uniqueIds_mapOp_def  uniqueIds_registerOp_def 
+        split: if_splits)[1])?;
+    ((rule procedure_cannot_guess_ids.intros, force); show_procedures_cannot_guess_ids?)?)
 
 
 end
